Make fault tolerance machinery ISA-generic

Picinae_riscv.v
@@ -539,33 +539,32 @@ Proof.
     exists rvtypctx. apply welltyped_rv2il.
 Qed.
 
-Definition inject_fault (p : program) (s : store) (a : addr) :=
-  match p s a with
-  | None => None
-  | Some (sz,q) => Some (sz,
-    If (BinOp OP_AND (BinOp OP_LT (Word 0x0 32) (Var V_FC)) (Unknown 1))
-      (Move V_FC (BinOp OP_MINUS (Var V_FC) (Word 0x1 32)))
-      q)
-  end.
+Require Import Picinae_fault_tolerance.
 
-Require Import Lia.
-Lemma inject_fault_lift_riscv_welltyped : forall p,
-    welltyped_prog rvtypctx (inject_fault (lift_riscv p)).
-Proof.
-    intros p s a. unfold inject_fault, lift_riscv.
-    exists rvtypctx.
-    econstructor.
-    change 1 with (widthof_binop OP_AND 1). constructor.
-        change 1 with (widthof_binop OP_LT 32). constructor.
-        constructor. lia. constructor. reflexivity.
-        constructor.
-    econstructor. now right.
-        change 32 with (widthof_binop OP_MINUS 32). constructor.
-        now constructor.
-        constructor. lia.
-        eapply typchk_stmt_mono with (c := rvtypctx) (c0 := rvtypctx)
-            (q := Move V_FC (BinOp OP_MINUS (Var V_FC) (Word 1 32))).
-        reflexivity. reflexivity.
-    apply welltyped_rv2il.
+Module FTC <: FaultToleranceConfig RISCVArch IL_RISCV.
+  Definition fault_counter := V_FC.
+  Theorem fault_counter_typed :
+        exists w,
+            1 < 2^w /\
+            archtyps fault_counter = Some w.
+  Proof.
+    exists 32. split. constructor.
     reflexivity.
+  Qed.
+End FTC.
+
+Module RVFaultTolerance := FaultTolerance RISCVArch
+                                          IL_RISCV
+                                          FTC
+                                          Theory_RISCV
+                                          Statics_RISCV.
+Import FTC RVFaultTolerance.
+
+Lemma inject_fault_lift_riscv_welltyped : forall p,
+  welltyped_prog rvtypctx (inject_fault (lift_riscv p)).
+Proof.
+  intros. apply inject_fault_welltyped.
+  intros. unfold lift_riscv in H. inversion H; subst; clear H.
+  apply welltyped_rv2il.
 Qed.
+
