Examples/crypto_memcmp/crypto_memcmp_proof.v
@@ -1,5 +1,6 @@
 Require Import memcmp_ft.
 Require Import Picinae_riscv.
+Import RVFaultTolerance.
 Import RISCVNotations.
 Require Import NArith.
 Require Import List.
