Picinae_fault_tolerance.v
@@ -1,0 +1,63 @@
+Require Import Picinae_core Picinae_statics Picinae_theory.
+Require Import NArith.
+
+Module Type FaultToleranceConfig (Arch : Architecture)
+                                 (IL : PICINAE_IL).
+    Import IL.
+    Parameter fault_counter : var.
+    Parameter fault_counter_typed :
+        exists w,
+            1 < 2^w /\
+            archtyps fault_counter = Some w.
+End FaultToleranceConfig.
+
+Module FaultTolerance (Arch : Architecture)
+                      (IL : PICINAE_IL)
+                      (FTC : FaultToleranceConfig Arch IL)
+                      (TIL : PICINAE_THEORY IL)
+                      (SIL : PICINAE_STATICS IL TIL).
+Import Arch IL FTC TIL SIL.
+
+Definition inject_fault (p : program) (s : store) (a : addr) :=
+  match p s a with
+  | None => None
+  | Some (sz,q) =>
+        match archtyps fault_counter with None => None | Some w =>
+        Some (sz,
+              If (BinOp OP_AND (BinOp OP_LT (Word 0x0 w) (Var fault_counter)) (Unknown 1))
+                (Move fault_counter (BinOp OP_MINUS (Var fault_counter) (Word 0x1 w)))
+              q)
+        end
+  end.
+
+Lemma inject_fault_welltyped : forall p,
+    (forall s a sz instr,
+        p s a = Some (sz, instr) ->
+        hastyp_stmt archtyps archtyps instr archtyps) ->
+    welltyped_prog archtyps (inject_fault p).
+Proof.
+    intros p WT s a. unfold inject_fault.
+    destruct (p s a) eqn:E; [|exact I]. destruct p0 as (sz & instr).
+    destruct fault_counter_typed as (w & BigW & FCW). rewrite FCW.
+    exists archtyps.
+    econstructor.
+    change 1 with (widthof_binop OP_AND 1). constructor.
+        change 1 with (widthof_binop OP_LT w). constructor.
+        constructor. apply mp2_gt_0. constructor. assumption.
+        constructor.
+    econstructor. right. eassumption.
+        change w with (widthof_binop OP_MINUS w) at 2. constructor.
+        now constructor.
+        constructor. assumption.
+        eapply typchk_stmt_mono with (c := archtyps) (c0 := archtyps)
+            (q := Move fault_counter (BinOp OP_MINUS (Var fault_counter) (Word 1 w))).
+            simpl. rewrite FCW. replace (1 <? 2^w) with true. rewrite N.eqb_refl.
+            pose proof (iseq_refl w). destruct H.
+                now replace (w == w) with (@left (w=w) (w<>w) x).
+            symmetry. now apply N.ltb_lt.
+        reflexivity.
+    eapply WT, E.
+    reflexivity.
+Qed.
+
+End FaultTolerance.
